specs/lean/Synchronicity/TrieProgramTests.lean
@@ -32,9 +32,9 @@ private def run : List (Reply (Option ByteArray)) → Program Storage (Reply Loo
   | _ :: _, .request .begin _ => none
   | _ :: _, .request (.commit _) _ => none
   | _ :: _, .request (.rollback _) _ => none
-  | _ :: _, .request (.readRows _ _ _ _) _ => none
+  | _ :: _, .request (.readRows _ _ _ _ _) _ => none
   | _ :: _, .request (.upsert _ _ _ _ _) _ => none
-  | _ :: _, .request (.deleteRows _ _ _) _ => none
+  | _ :: _, .request (.deleteRows _ _ _ _) _ => none
   | _ :: _, .request (.readInput _ _ _) _ => none
   | _ :: _, .request (.readCounter _ _) _ => none
   | _ :: _, .request (.removeFile _ _) _ => none
